IMPminus_TM/GOTO_WHILE/GOTO_Instr_to_While_Prog.thy
@@ -4,17 +4,17 @@ begin
 
 fun well_defined_instr :: "instr \<Rightarrow> bool" where
   "well_defined_instr HALT = True" | 
-  "well_defined_instr (x ::= t) = (x \<noteq> ''pc''\<and> (case t of N c \<Rightarrow> True | V y \<Rightarrow> y \<noteq> ''pc''))" |
+  "well_defined_instr (x ;;= t) = (x \<noteq> ''pc''\<and> (case t of N c \<Rightarrow> True | V y \<Rightarrow> y \<noteq> ''pc''))" |
   "well_defined_instr (x += t) = (x \<noteq> ''pc''\<and> (case t of N c \<Rightarrow> True | V y \<Rightarrow> y \<noteq> ''pc''))" |
   "well_defined_instr (x -= t) = (x \<noteq> ''pc'' \<and> (case t of N c \<Rightarrow> True | V y \<Rightarrow> y \<noteq> ''pc''))" |
   "well_defined_instr (x \<bind>1) = (x \<noteq> ''pc'')" |
   "well_defined_instr (x %=2) = (x \<noteq> ''pc'')" |
   "well_defined_instr (GOTO i) = (i > 0)" |
-  "well_defined_instr (IF x\<noteq>0 THEN GOTO i) = (x \<noteq> ''pc'')"
+  "well_defined_instr (IF x\<noteq>0 THEN GOTO i) = (x \<noteq> ''pc'' \<and> i > 0)"
 
 fun GOTO_Instr_to_WHILE :: "instr \<Rightarrow> com" where
   "GOTO_Instr_to_WHILE HALT = ''pc'' ::= A (atomExp.N 0)" | 
-  "GOTO_Instr_to_WHILE (x ::= t) = 
+  "GOTO_Instr_to_WHILE (x ;;= t) = 
     (case t of operi.N c \<Rightarrow> x ::= A (atomExp.N c) | operi.V y \<Rightarrow> x ::= A (atomExp.V y)) ;; 
     ''pc'' ::= (atomExp.V ''pc'' \<oplus> atomExp.N 1)" | 
   "GOTO_Instr_to_WHILE (x += t) = 
@@ -31,6 +31,46 @@ fun GOTO_Instr_to_WHILE :: "instr \<Rightarrow> com" where
     ''pc'' ::= (atomExp.V ''pc'' \<oplus> atomExp.N 1)" | 
   "GOTO_Instr_to_WHILE (GOTO i) = ''pc'' ::= A (atomExp.N i)" | 
   "GOTO_Instr_to_WHILE (IF x\<noteq>0 THEN GOTO i) = IF x\<noteq>0 THEN ''pc'' ::= A (atomExp.N i) ELSE ''pc'' ::= (atomExp.V ''pc'' \<oplus> atomExp.N 1)"
+
+lemma instr_halt_complexity:
+  "\<exists>t. (GOTO_Instr_to_WHILE HALT, s) \<Rightarrow>\<^bsup> 2 \<^esup> t"
+  by (metis AssignI' GOTO_Instr_to_WHILE.simps(1))
+
+lemma instr_assign_complexity:
+  "\<exists>t. (GOTO_Instr_to_WHILE (x ;;= c), s) \<Rightarrow>\<^bsup> 4 \<^esup> t"
+  apply (cases c)
+  apply fastforce
+  by fastforce
+
+lemma instr_add_complexity:
+  "\<exists>t. (GOTO_Instr_to_WHILE (x += c), s) \<Rightarrow>\<^bsup> 4 \<^esup> t"
+  apply (cases c)
+  apply fastforce
+  by fastforce
+
+lemma instr_sub_complexity:
+  "\<exists>t. (GOTO_Instr_to_WHILE (x -= c), s) \<Rightarrow>\<^bsup> 4 \<^esup> t"
+  apply (cases c)
+  apply fastforce
+  by fastforce
+
+lemma instr_right_shift_complexity:
+  "\<exists>t. (GOTO_Instr_to_WHILE (x \<bind>1), s) \<Rightarrow>\<^bsup> 4 \<^esup> t"
+  by fastforce
+
+lemma instr_left_shift_complexity:
+  "\<exists>t. (GOTO_Instr_to_WHILE (x %=2), s) \<Rightarrow>\<^bsup> 4 \<^esup> t"
+  by fastforce
+
+lemma instr_jump_complexity:
+  "\<exists>t. (GOTO_Instr_to_WHILE (GOTO i), s) \<Rightarrow>\<^bsup> 2 \<^esup> t"
+  by (metis AssignI'' GOTO_Instr_to_WHILE.simps(7))
+
+lemma instr_cond_jump_complexity:
+  "\<exists>t. (GOTO_Instr_to_WHILE (IF x\<noteq>0 THEN GOTO i), s) \<Rightarrow>\<^bsup> 3 \<^esup> t"
+  apply (cases "s x")
+  apply fastforce
+  by fastforce
 
 lemma instr_pc_consist:
   assumes "well_defined_instr instr"
@@ -62,7 +102,7 @@ next
     hence "t = ?inter(''pc'' := ?inter ''pc'' + 1)" using ASSIGN N assms(2) by auto
     hence aux3: "t ''pc'' = pc + 1" using ASSIGN assms(1) assms(4) by auto
 
-    have "iexec (x ::= tmp) (pc, s') = (pc + 1, s'(x := c))" by (simp add: N)
+    have "iexec (x ;;= tmp) (pc, s') = (pc + 1, s'(x := c))" by (simp add: N)
     hence aux4: "pc' = pc + 1" using ASSIGN assms(3) by auto
 
     show ?thesis using aux3 aux4 by blast
@@ -77,7 +117,7 @@ next
     hence "t = ?inter(''pc'' := ?inter ''pc'' + 1)" using ASSIGN V assms(2) by auto
     hence aux3: "t ''pc'' = pc + 1" using ASSIGN assms(1) assms(4) by auto
 
-    have "iexec (x ::= tmp) (pc, s') = (pc + 1, s'(x := s' y))" by (simp add: V)
+    have "iexec (x ;;= tmp) (pc, s') = (pc + 1, s'(x := s' y))" by (simp add: V)
     hence aux4: "pc' = pc + 1" using ASSIGN assms(3) by auto
 
     show ?thesis using aux3 aux4 by blast
@@ -244,7 +284,7 @@ next
     have "(?w_com, s) \<Rightarrow>\<^bsup> 4 \<^esup> ?inter(''pc'' := ?inter ''pc'' + 1)" using aux1 aux2 by (simp add: Seq)
     hence aux3: "t = ?inter(''pc'' := ?inter ''pc'' + 1)" using ASSIGN N assms(2) by auto
 
-    have "iexec (x ::= tmp) (pc, s') = (pc + 1, s'(x := c))" by (simp add: N)
+    have "iexec (x ;;= tmp) (pc, s') = (pc + 1, s'(x := c))" by (simp add: N)
     hence aux4: "t' = s'(x := c)" using ASSIGN assms(3) by auto
 
     show ?thesis using aux3 aux4 by (simp add: assms(5))
@@ -258,7 +298,7 @@ next
     have "(?w_com, s) \<Rightarrow>\<^bsup> 4 \<^esup> ?inter(''pc'' := ?inter ''pc'' + 1)" using aux1 aux2 by (simp add: Seq)
     hence aux3: "t = ?inter(''pc'' := ?inter ''pc'' + 1)" using ASSIGN V assms(2) by auto
 
-    have "iexec (x ::= tmp) (pc, s') = (pc + 1, s'(x := s' y))" by (simp add: V)
+    have "iexec (x ;;= tmp) (pc, s') = (pc + 1, s'(x := s' y))" by (simp add: V)
     hence aux4: "t' = s'(x := s' y)" using ASSIGN assms(3) by auto
 
     let ?inter' = "s'(x := s' y)"
@@ -403,8 +443,130 @@ theorem single_instr_consist:
     and "(GOTO_Instr_to_WHILE instr, s) \<Rightarrow>\<^bsup> k \<^esup> t"
     and "iexec instr (pc, s') = (pc', t')" 
     and "s ''pc'' = pc" and "\<forall>x \<noteq> ''pc''. s x = s' x"
-  shows "t ''pc'' = pc'" and "\<forall>x \<noteq> ''pc''. t x = t' x"
+  shows "t ''pc'' = pc'" and "\<forall>x \<noteq> ''pc''. t x = t' x" 
   using assms(1) assms(2) assms(3) assms(4) assms(5) instr_pc_consist apply auto[1]
   using assms(1) assms(2) assms(3) assms(4) assms(5) instr_var_consist by presburger
+
+lemma "(GOTO_Instr_to_WHILE HALT, s) \<Rightarrow>\<^bsup> 2 \<^esup> t" using instr_halt_complexity sorry
+
+theorem instr_halt:
+  assumes "well_defined_instr HALT"
+  and "iexec HALT (pc, s') = (pc', t')"
+  and "s ''pc'' = pc" and "\<forall>x \<noteq> ''pc''. s x = s' x"
+  shows "\<exists>t. ((GOTO_Instr_to_WHILE HALT, s) \<Rightarrow>\<^bsup> 2 \<^esup> t) \<and> (t ''pc'' = pc') \<and> (\<forall>x \<noteq> ''pc''. t x = t' x)" using assms
+proof -
+  have "\<exists>t. (GOTO_Instr_to_WHILE HALT, s) \<Rightarrow>\<^bsup> 2 \<^esup> t" using instr_halt_complexity by blast
+  then obtain t where aux: "(GOTO_Instr_to_WHILE HALT, s) \<Rightarrow>\<^bsup> 2 \<^esup> t" by blast
+  hence "(t ''pc'' = pc') \<and> (\<forall>x \<noteq> ''pc''. t x = t' x)" using assms by (meson instr_pc_consist instr_var_consist) 
+  thus "\<exists>t. ((GOTO_Instr_to_WHILE HALT, s) \<Rightarrow>\<^bsup> 2 \<^esup> t) \<and> (t ''pc'' = pc') \<and> (\<forall>x \<noteq> ''pc''. t x = t' x)" using aux by blast
+qed
+
+lemma instr_complexity_halt':
+  "(GOTO_Instr_to_WHILE HALT, s) \<Rightarrow>\<^bsup> k \<^esup> t \<Longrightarrow> k = 2" by (meson bigstep_det instr_halt_complexity)
+
+theorem instr_assign:
+  assumes "well_defined_instr (x ;;= c)"
+  and "iexec (x ;;= c) (pc, s') = (pc', t')"
+  and "s ''pc'' = pc" and "\<forall>x \<noteq> ''pc''. s x = s' x"
+  shows "\<exists>t. ((GOTO_Instr_to_WHILE (x ;;= c), s) \<Rightarrow>\<^bsup> 4 \<^esup> t) \<and> (t ''pc'' = pc') \<and> (\<forall>x \<noteq> ''pc''. t x = t' x)" using assms
+proof -
+  have "\<exists>t. (GOTO_Instr_to_WHILE (x ;;= c), s) \<Rightarrow>\<^bsup> 4 \<^esup> t" using instr_assign_complexity by blast
+  then obtain t where aux: "(GOTO_Instr_to_WHILE (x ;;= c), s) \<Rightarrow>\<^bsup> 4 \<^esup> t" by blast
+  hence "(t ''pc'' = pc') \<and> (\<forall>x \<noteq> ''pc''. t x = t' x)" using assms by (meson instr_pc_consist instr_var_consist) 
+  thus "\<exists>t. ((GOTO_Instr_to_WHILE (x ;;= c), s) \<Rightarrow>\<^bsup> 4 \<^esup> t) \<and> (t ''pc'' = pc') \<and> (\<forall>x \<noteq> ''pc''. t x = t' x)" using aux by blast
+qed
+
+lemma instr_complexity_assign':
+  "(GOTO_Instr_to_WHILE (x ;;= c), s) \<Rightarrow>\<^bsup> k \<^esup> t \<Longrightarrow> k = 4" by (meson bigstep_det instr_assign_complexity)
+
+theorem instr_add:
+  assumes "well_defined_instr (x += c)"
+  and "iexec (x += c) (pc, s') = (pc', t')"
+  and "s ''pc'' = pc" and "\<forall>x \<noteq> ''pc''. s x = s' x"
+  shows "\<exists>t. ((GOTO_Instr_to_WHILE (x += c), s) \<Rightarrow>\<^bsup> 4 \<^esup> t) \<and> (t ''pc'' = pc') \<and> (\<forall>x \<noteq> ''pc''. t x = t' x)" using assms
+proof -
+  have "\<exists>t. (GOTO_Instr_to_WHILE (x += c), s) \<Rightarrow>\<^bsup> 4 \<^esup> t" using instr_add_complexity by blast
+  then obtain t where aux: "(GOTO_Instr_to_WHILE (x += c), s) \<Rightarrow>\<^bsup> 4 \<^esup> t" by blast
+  hence "(t ''pc'' = pc') \<and> (\<forall>x \<noteq> ''pc''. t x = t' x)" using assms by (meson instr_pc_consist instr_var_consist) 
+  thus "\<exists>t. ((GOTO_Instr_to_WHILE (x += c), s) \<Rightarrow>\<^bsup> 4 \<^esup> t) \<and> (t ''pc'' = pc') \<and> (\<forall>x \<noteq> ''pc''. t x = t' x)" using aux by blast
+qed
+
+lemma instr_complexity_add':
+  "(GOTO_Instr_to_WHILE (x += c), s) \<Rightarrow>\<^bsup> k \<^esup> t \<Longrightarrow> k = 4" by (meson bigstep_det instr_add_complexity)
+
+theorem instr_sub:
+  assumes "well_defined_instr (x -= c)"
+  and "iexec (x -= c) (pc, s') = (pc', t')"
+  and "s ''pc'' = pc" and "\<forall>x \<noteq> ''pc''. s x = s' x"
+  shows "\<exists>t. ((GOTO_Instr_to_WHILE (x -= c), s) \<Rightarrow>\<^bsup> 4 \<^esup> t) \<and> (t ''pc'' = pc') \<and> (\<forall>x \<noteq> ''pc''. t x = t' x)" using assms
+proof -
+  have "\<exists>t. (GOTO_Instr_to_WHILE (x -= c), s) \<Rightarrow>\<^bsup> 4 \<^esup> t" using instr_sub_complexity by blast
+  then obtain t where aux: "(GOTO_Instr_to_WHILE (x -= c), s) \<Rightarrow>\<^bsup> 4 \<^esup> t" by blast
+  hence "(t ''pc'' = pc') \<and> (\<forall>x \<noteq> ''pc''. t x = t' x)" using assms by (meson instr_pc_consist instr_var_consist) 
+  thus "\<exists>t. ((GOTO_Instr_to_WHILE (x -= c), s) \<Rightarrow>\<^bsup> 4 \<^esup> t) \<and> (t ''pc'' = pc') \<and> (\<forall>x \<noteq> ''pc''. t x = t' x)" using aux by blast
+qed
+
+lemma instr_complexity_sub':
+  "(GOTO_Instr_to_WHILE (x -= c), s) \<Rightarrow>\<^bsup> k \<^esup> t \<Longrightarrow> k = 4" by (meson bigstep_det instr_sub_complexity)
+
+theorem instr_right_shift:
+  assumes "well_defined_instr (x \<bind>1)"
+  and "iexec (x \<bind>1) (pc, s') = (pc', t')"
+  and "s ''pc'' = pc" and "\<forall>x \<noteq> ''pc''. s x = s' x"
+  shows "\<exists>t. ((GOTO_Instr_to_WHILE (x \<bind>1), s) \<Rightarrow>\<^bsup> 4 \<^esup> t) \<and> (t ''pc'' = pc') \<and> (\<forall>x \<noteq> ''pc''. t x = t' x)" using assms
+proof -
+  have "\<exists>t. (GOTO_Instr_to_WHILE (x \<bind>1), s) \<Rightarrow>\<^bsup> 4 \<^esup> t" using instr_right_shift_complexity by blast
+  then obtain t where aux: "(GOTO_Instr_to_WHILE (x \<bind>1), s) \<Rightarrow>\<^bsup> 4 \<^esup> t" by blast
+  hence "(t ''pc'' = pc') \<and> (\<forall>x \<noteq> ''pc''. t x = t' x)" using assms by (meson instr_pc_consist instr_var_consist) 
+  thus "\<exists>t. ((GOTO_Instr_to_WHILE (x \<bind>1), s) \<Rightarrow>\<^bsup> 4 \<^esup> t) \<and> (t ''pc'' = pc') \<and> (\<forall>x \<noteq> ''pc''. t x = t' x)" using aux by blast
+qed
+
+lemma instr_complexity_right_shift':
+  "(GOTO_Instr_to_WHILE (x \<bind>1), s) \<Rightarrow>\<^bsup> k \<^esup> t \<Longrightarrow> k = 4" by (meson bigstep_det instr_right_shift_complexity)
+
+theorem instr_left_shift:
+  assumes "well_defined_instr (x %=2)"
+  and "iexec (x %=2) (pc, s') = (pc', t')"
+  and "s ''pc'' = pc" and "\<forall>x \<noteq> ''pc''. s x = s' x"
+  shows "\<exists>t. ((GOTO_Instr_to_WHILE (x %=2), s) \<Rightarrow>\<^bsup> 4 \<^esup> t) \<and> (t ''pc'' = pc') \<and> (\<forall>x \<noteq> ''pc''. t x = t' x)" using assms
+proof -
+  have "\<exists>t. (GOTO_Instr_to_WHILE (x %=2), s) \<Rightarrow>\<^bsup> 4 \<^esup> t" using instr_left_shift_complexity by blast
+  then obtain t where aux: "(GOTO_Instr_to_WHILE (x %=2), s) \<Rightarrow>\<^bsup> 4 \<^esup> t" by blast
+  hence "(t ''pc'' = pc') \<and> (\<forall>x \<noteq> ''pc''. t x = t' x)" using assms by (meson instr_pc_consist instr_var_consist) 
+  thus "\<exists>t. ((GOTO_Instr_to_WHILE (x %=2), s) \<Rightarrow>\<^bsup> 4 \<^esup> t) \<and> (t ''pc'' = pc') \<and> (\<forall>x \<noteq> ''pc''. t x = t' x)" using aux by blast
+qed
+
+lemma instr_complexity_left_shift':
+  "(GOTO_Instr_to_WHILE (x %=2), s) \<Rightarrow>\<^bsup> k \<^esup> t \<Longrightarrow> k = 4" by (meson bigstep_det instr_left_shift_complexity)
+
+theorem instr_jump:
+  assumes "well_defined_instr (GOTO i)"
+  and "iexec (GOTO i) (pc, s') = (pc', t')"
+  and "s ''pc'' = pc" and "\<forall>x \<noteq> ''pc''. s x = s' x"
+  shows "\<exists>t. ((GOTO_Instr_to_WHILE (GOTO i), s) \<Rightarrow>\<^bsup> 2 \<^esup> t) \<and> (t ''pc'' = pc') \<and> (\<forall>x \<noteq> ''pc''. t x = t' x)" using assms
+proof -
+  have "\<exists>t. (GOTO_Instr_to_WHILE (GOTO i), s) \<Rightarrow>\<^bsup> 2 \<^esup> t" using instr_jump_complexity by blast
+  then obtain t where aux: "(GOTO_Instr_to_WHILE (GOTO i), s) \<Rightarrow>\<^bsup> 2 \<^esup> t" by blast
+  hence "(t ''pc'' = pc') \<and> (\<forall>x \<noteq> ''pc''. t x = t' x)" using assms by (meson instr_pc_consist instr_var_consist) 
+  thus "\<exists>t. ((GOTO_Instr_to_WHILE (GOTO i), s) \<Rightarrow>\<^bsup> 2 \<^esup> t) \<and> (t ''pc'' = pc') \<and> (\<forall>x \<noteq> ''pc''. t x = t' x)" using aux by blast
+qed
+
+lemma instr_complexity_jump':
+  "(GOTO_Instr_to_WHILE (GOTO i), s) \<Rightarrow>\<^bsup> k \<^esup> t \<Longrightarrow> k = 2" by (meson bigstep_det instr_jump_complexity)
+
+theorem instr_cond_jump:
+  assumes "well_defined_instr (IF x\<noteq>0 THEN GOTO i)"
+  and "iexec (IF x\<noteq>0 THEN GOTO i) (pc, s') = (pc', t')"
+  and "s ''pc'' = pc" and "\<forall>x \<noteq> ''pc''. s x = s' x"
+  shows "\<exists>t. ((GOTO_Instr_to_WHILE (IF x\<noteq>0 THEN GOTO i), s) \<Rightarrow>\<^bsup> 3 \<^esup> t) \<and> (t ''pc'' = pc') \<and> (\<forall>x \<noteq> ''pc''. t x = t' x)" using assms
+proof -
+  have "\<exists>t. (GOTO_Instr_to_WHILE (IF x\<noteq>0 THEN GOTO i), s) \<Rightarrow>\<^bsup> 3 \<^esup> t" using instr_cond_jump_complexity by blast
+  then obtain t where aux: "(GOTO_Instr_to_WHILE (IF x\<noteq>0 THEN GOTO i), s) \<Rightarrow>\<^bsup> 3 \<^esup> t" by blast
+  hence "(t ''pc'' = pc') \<and> (\<forall>x \<noteq> ''pc''. t x = t' x)" using assms by (meson instr_pc_consist instr_var_consist) 
+  thus "\<exists>t. ((GOTO_Instr_to_WHILE (IF x\<noteq>0 THEN GOTO i), s) \<Rightarrow>\<^bsup> 3 \<^esup> t) \<and> (t ''pc'' = pc') \<and> (\<forall>x \<noteq> ''pc''. t x = t' x)" using aux by blast
+qed
+
+lemma instr_complexity_cond_jump':
+  "(GOTO_Instr_to_WHILE (IF x\<noteq>0 THEN GOTO i), s) \<Rightarrow>\<^bsup> k \<^esup> t \<Longrightarrow> k = 3" by (meson bigstep_det instr_cond_jump_complexity)
 
 end
