IMPminus_TM/GOTO_WHILE/GOTO_Prog_to_While_Prog.thy
@@ -114,7 +114,7 @@ termination apply (relation "measure (\<lambda>(prog, t) . length prog + 1 - t)"
 definition GOTO_Prog_to_WHILE_IF :: "GOTO_Prog \<Rightarrow> com" where 
   "GOTO_Prog_to_WHILE_IF prog = GOTO_Prog_to_WHILE_IF' prog 1"
 
-value "GOTO_Prog_to_WHILE_IF [''x'' ::= N 3, ''y'' ::= N 4, ''z'' ::= V ''x'', ''z'' += V ''y'', HALT]"
+value "GOTO_Prog_to_WHILE_IF [''x'' ;;= N 3, ''y'' ;;= N 4, ''z'' ;;= V ''x'', ''z'' += V ''y'', HALT]"
 
 lemma GOTO_Prog_to_WHILE_IF'_correctness_complexity:
   assumes "1 \<le> min_pc" and "min_pc \<le> pc" and "pc \<le> length prog" and "s ''pc'' = pc"
@@ -144,23 +144,447 @@ lemma GOTO_Prog_to_WHILE_IF_correctness_complexity:
   shows "(GOTO_Prog_to_WHILE_IF prog, s) \<Rightarrow>\<^bsup> i + s ''pc'' * 5 \<^esup> t" using assms
   by (metis GOTO_Prog_to_WHILE_IF'_correctness_complexity GOTO_Prog_to_WHILE_IF_def add.commute diff_Suc_1 less_or_eq_imp_le plus_1_eq_Suc)
 
+lemma GOTO_Prog_to_WHILE_IF_correctness_complexity':
+  assumes "1 \<le> s ''pc''" and "s ''pc'' \<le> length prog"
+    and "\<exists>t. (GOTO_Instr_to_WHILE (prog !! s ''pc''), s) \<Rightarrow>\<^bsup> i \<^esup> t"
+  shows "\<exists>t. (GOTO_Prog_to_WHILE_IF prog, s) \<Rightarrow>\<^bsup> i + s ''pc'' * 5 \<^esup> t" using assms
+  using GOTO_Prog_to_WHILE_IF_correctness_complexity by blast
+
 definition GOTO_Prog_to_WHILE :: "GOTO_Prog \<Rightarrow> com" where
   "GOTO_Prog_to_WHILE prog = ''pc'' ::= A (atomExp.N 1) ;; WHILE ''pc''\<noteq>0 DO GOTO_Prog_to_WHILE_IF prog"
 
-definition well_defined_prog :: "GOTO_Prog \<Rightarrow> bool" where
-  "well_defined_prog prog = (\<forall>i. (1 \<le> i \<and> i \<le> length prog) \<longrightarrow> (well_defined_instr (prog !! i)))"
+(*reversed version necessary !!! *)
+lemma GOTO_Prog_to_WHILE_IF'_correctness_complexity_reversed:
+  assumes "1 \<le> min_pc" and "min_pc \<le> pc" and "pc \<le> length prog" and "s ''pc'' = pc"
+    and "(GOTO_Prog_to_WHILE_IF' prog min_pc, s) \<Rightarrow>\<^bsup> i + (pc + 1 - min_pc) * 5 \<^esup> t"
+  shows "(GOTO_Instr_to_WHILE (prog !! pc), s) \<Rightarrow>\<^bsup> i \<^esup> t" using assms
+proof (induction prog min_pc arbitrary: rule: GOTO_Prog_to_WHILE_IF'.induct)
+  case (1 prog min_pc)
+  consider (c1) "min_pc = pc" | (c2) "min_pc < pc" using "1.prems"(2) by linarith
+  then show ?case using 1
+  proof cases
+    case c1
+    have "(GOTO_Instr_to_WHILE (prog !! pc), s) \<Rightarrow>\<^bsup> i \<^esup> t"
+      by (metis "1.prems"(3) "1.prems"(5) GOTO_Prog_to_WHILE_IF'.elims add_diff_cancel_left' assms(4) c1 if_neq_trans_out_2_ins_eq lambda_one verit_comp_simplify1(3))
+    thus ?thesis using 1 c1 by simp
+  next
+    case c2
+    thm if_neq_trans_out_2_ins_gt
+    show ?thesis using c2 1 if_neq_trans_out_2_ins_gt
+      by (smt (verit, ccfv_threshold) GOTO_Prog_to_WHILE_IF'.elims Suc_diff_le Suc_eq_plus1 add.commute add.left_commute add_diff_cancel_right' diff_diff_left less_eq_Suc_le mult_Suc nat_less_le not_less_eq_eq order_less_le_trans)
+  qed
+qed
 
-(*
+lemma GOTO_Prog_to_WHILE_IF_correctness_complexity_reversed:
+  assumes "1 \<le> s ''pc''" and "s ''pc'' \<le> length prog"
+    and "(GOTO_Prog_to_WHILE_IF prog, s) \<Rightarrow>\<^bsup> i + s ''pc'' * 5 \<^esup> t"
+  shows "(GOTO_Instr_to_WHILE (prog !! s ''pc''), s) \<Rightarrow>\<^bsup> i \<^esup> t" using assms
+  by (metis GOTO_Prog_to_WHILE_IF'_correctness_complexity_reversed GOTO_Prog_to_WHILE_IF_def add.commute add_diff_cancel_left' le_refl)
+
 definition well_defined_prog :: "GOTO_Prog \<Rightarrow> bool" where
-  "well_defined_prog prog = (\<forall>i. (1 \<le> i \<and> i \<le> length prog) \<longrightarrow> 
-    (well_defined_instr (prog !! i) \<and> (case prog !! i of GOTO j \<Rightarrow> j \<le> length prog | _ \<Rightarrow> True)))"
-*)
+  "well_defined_prog prog = (length prog \<ge> 1 \<and> (\<forall>i. (1 \<le> i \<and> i \<le> length prog) \<longrightarrow> (
+    well_defined_instr (prog !! i) \<and> 
+    (case prog !! i of GOTO j \<Rightarrow> j \<le> length prog | IF x\<noteq>0 THEN GOTO j \<Rightarrow> j \<le> length prog | _ \<Rightarrow> True) \<and> 
+    prog !! (length prog) = HALT)
+  ))"
+
+lemma well_defined_prog_pc_range:
+  assumes "prog \<turnstile> (pc, s) \<rightarrow>\<^bsup> k \<^esup> (pc', t)"
+    and "well_defined_prog prog"
+    and "1 \<le> pc \<and> pc \<le> length prog"
+  shows "0 \<le> pc' \<and> pc' \<le> length prog" using assms
+proof (induct prog pc s k pc' t rule: exec_t_induct)
+  case (step0 P pc s)
+  then show ?case by simp
+next
+  case (step1 P pc\<^sub>1 s\<^sub>1 pc\<^sub>2 s\<^sub>2 x pc\<^sub>3 s\<^sub>3)
+  have expand: "iexec (P !! pc\<^sub>1) (pc\<^sub>1, s\<^sub>1) = (pc\<^sub>2, s\<^sub>2)" using step1.hyps(1) exec1_def by auto
+  show ?case
+  proof (cases "P !! pc\<^sub>1")
+    case HALT
+    have "pc\<^sub>2 = 0" using HALT expand by auto
+    thus ?thesis using step1 HALT by blast
+  next
+    case (ASSIGN v op)
+    have "pc\<^sub>2 = pc\<^sub>1 + 1" using ASSIGN expand by auto
+    thus ?thesis using step1 ASSIGN
+      by (metis Suc_eq_plus1 instr.distinct(2) le_neq_implies_less less_eq_Suc_le trans_le_add1 well_defined_prog_def)
+  next
+    case (ADD v op)
+    have "pc\<^sub>2 = pc\<^sub>1 + 1" using ADD expand by auto
+    thus ?thesis using step1 ADD
+      by (metis Suc_eq_plus1 instr.distinct(4) le_neq_implies_less less_eq_Suc_le trans_le_add1 well_defined_prog_def)
+  next
+    case (SUB v op)
+    have "pc\<^sub>2 = pc\<^sub>1 + 1" using SUB expand by auto
+    thus ?thesis using step1 SUB
+      by (metis Suc_eq_plus1 instr.distinct(6) le_neq_implies_less less_eq_Suc_le trans_le_add1 well_defined_prog_def)
+  next
+    case (RSH v)
+    have "pc\<^sub>2 = pc\<^sub>1 + 1" using RSH expand by auto
+    thus ?thesis using step1 RSH
+      using less_eq_Suc_le well_defined_prog_def by fastforce
+  next
+    case (MOD v)
+    have "pc\<^sub>2 = pc\<^sub>1 + 1" using MOD expand by auto
+    thus ?thesis using step1 MOD
+      using less_eq_Suc_le well_defined_prog_def by fastforce
+  next
+    case (JMP i)
+    have "pc\<^sub>2 = i" using JMP expand by auto
+    have "i > 0" using step1.hyps(2) \<open>pc\<^sub>2 = i\<close> by fastforce
+    have "case P !! i of GOTO j \<Rightarrow> j \<le> length P | IF x\<noteq>0 THEN GOTO j \<Rightarrow> j \<le> length P | _ \<Rightarrow> True"
+      by (metis step1.prems(1) step1.prems(2) JMP One_nat_def \<open>0 < i\<close> instr.simps(70) less_eq_Suc_le well_defined_prog_def)
+    hence "i \<le> length P" using step1.prems(1) step1.prems(2) JMP well_defined_prog_def by auto
+    thus ?thesis using step1.hyps(2) step1.hyps(4) step1.prems(1) \<open>pc\<^sub>2 = i\<close> by force
+  next
+    case (CONDJMP v i)
+    consider (c1) "s\<^sub>1 v = 0" | (c2) "s\<^sub>1 v > 0" by blast
+    then show ?thesis
+    proof cases
+      case c1
+      have "pc\<^sub>2 = pc\<^sub>1 + 1" using CONDJMP expand c1 by auto
+      thus ?thesis using CONDJMP step1 c1
+        by (smt (verit) Suc_eq_plus1 instr.case(1) instr.case(8) less_Suc_eq_le less_or_eq_imp_le linorder_le_less_linear order_antisym well_defined_prog_def)
+    next
+      case c2
+      have "pc\<^sub>2 = i" using CONDJMP expand c2 by auto
+      have "i > 0" using step1.hyps(2) \<open>pc\<^sub>2 = i\<close> by fastforce
+      have "case P !! i of GOTO j \<Rightarrow> j \<le> length P | IF x\<noteq>0 THEN GOTO j \<Rightarrow> j \<le> length P | _ \<Rightarrow> True"
+        by (metis step1.prems(1) step1.prems(2) CONDJMP One_nat_def \<open>0 < i\<close> instr.simps(71) less_eq_Suc_le well_defined_prog_def)
+      hence "i \<le> length P" using step1.prems(1) step1.prems(2) CONDJMP well_defined_prog_def by auto
+      thus ?thesis using step1.hyps(4) step1.prems(1) \<open>0 < i\<close> \<open>pc\<^sub>2 = i\<close> by fastforce
+    qed
+  qed
+qed
+
+lemma well_defined_prog_pc_range_single:
+  assumes "prog \<turnstile> (pc, s) \<rightarrow> (pc', t)"
+    and "well_defined_prog prog"
+    and "1 \<le> pc \<and> pc \<le> length prog"
+  shows "0 \<le> pc' \<and> pc' \<le> length prog" using assms
+  by (metis exec_t.intros(1) exec_t.intros(2) well_defined_prog_pc_range zero_le)
+
+lemma prog_if_pc_consist:
+  assumes "prog \<turnstile> (pc, s') \<rightarrow> (pc', t')"
+    and "1 \<le> pc" and "pc \<le> length prog"
+    and "well_defined_prog prog"
+    and "(GOTO_Prog_to_WHILE_IF prog, s) \<Rightarrow>\<^bsup> i + s ''pc'' * 5 \<^esup> t"
+    and "s ''pc'' = pc" and "\<forall>x \<noteq> ''pc''. s x = s' x"
+  shows "t ''pc'' = pc'" using assms
+proof -
+  have pre2: "(GOTO_Instr_to_WHILE (prog !! s ''pc''), s) \<Rightarrow>\<^bsup> i \<^esup> t"
+    using GOTO_Prog_to_WHILE_IF_correctness_complexity_reversed assms(2) assms(3) assms(5) assms(6) by blast
+  have pre1: "well_defined_instr (prog !! s ''pc'')" using assms(2) assms(3) assms(4) assms(6) well_defined_prog_def by blast
+  have pre3: "iexec (prog !! s ''pc'') (pc, s') = (pc', t')" using assms(1) assms(6) exec1_def by auto
+  thus "t ''pc'' = pc'" using pre1 pre2 pre3 assms by (simp add: instr_pc_consist)
+qed
+
+lemma prog_if_var_consist:
+  assumes "prog \<turnstile> (pc, s') \<rightarrow> (pc', t')"
+    and "1 \<le> pc" and "pc \<le> length prog"
+    and "well_defined_prog prog"
+    and "(GOTO_Prog_to_WHILE_IF prog, s) \<Rightarrow>\<^bsup> i + s ''pc'' * 5 \<^esup> t"
+    and "s ''pc'' = pc" and "\<forall>x \<noteq> ''pc''. s x = s' x"
+  shows "\<forall>z \<noteq> ''pc''. t z = t' z" using assms
+proof -
+  have pre2: "(GOTO_Instr_to_WHILE (prog !! s ''pc''), s) \<Rightarrow>\<^bsup> i \<^esup> t"
+    using GOTO_Prog_to_WHILE_IF_correctness_complexity_reversed assms(2) assms(3) assms(5) assms(6) by blast
+  have pre1: "well_defined_instr (prog !! s ''pc'')" using assms(2) assms(3) assms(4) assms(6) well_defined_prog_def by blast
+  have pre3: "iexec (prog !! s ''pc'') (pc, s') = (pc', t')" using assms(1) assms(6) exec1_def by auto
+  thus "\<forall>z \<noteq> ''pc''. t z = t' z" using pre1 pre2 pre3 assms by (simp add: instr_var_consist)
+qed
+
+fun WHILE_complexity :: "GOTO_Prog \<Rightarrow> config \<Rightarrow> nat \<Rightarrow> nat" where
+  "WHILE_complexity _ _ 0 = 0" | 
+  "WHILE_complexity prog (pc, s) (Suc step) = WHILE_complexity prog (iexec (prog !! pc) (pc, s)) step + 5 * pc + 1 + 
+    (case (prog !! pc) of 
+      HALT \<Rightarrow> 2 |
+      x ;;= t \<Rightarrow> 4 |
+      x += t \<Rightarrow> 4 | 
+      x -= t \<Rightarrow> 4 | 
+      x \<bind>1 \<Rightarrow> 4 |
+      x %=2 \<Rightarrow> 4 |
+      GOTO i \<Rightarrow> 2 | 
+      IF x\<noteq>0 THEN GOTO i \<Rightarrow> 3
+    )"
+
+lemma "(com1;;com2, s1) \<Rightarrow>\<^bsup> c \<^esup> s3 \<Longrightarrow> (com1, s1) \<Rightarrow>\<^bsup> c1 \<^esup> s2 \<Longrightarrow> (com2, s2) \<Rightarrow>\<^bsup> c - c1 \<^esup> s3"
+  using bigstep_det by fastforce
+
+lemma "(WHILE b \<noteq>0 DO c, s1) \<Rightarrow>\<^bsup> z \<^esup> s3 \<Longrightarrow> s1 b \<noteq> 0 \<Longrightarrow> (c,s1) \<Rightarrow>\<^bsup> x \<^esup> s2 \<Longrightarrow> (WHILE b \<noteq>0 DO c, s2) \<Rightarrow>\<^bsup> z - x - 1 \<^esup> s3"
+  by (smt (verit) One_nat_def While_tE_time add.commute add_0 add_diff_cancel_left' bigstep_det diff_Suc_Suc diff_diff_eq)
 
 lemma prog_pc_consist:
-  assumes "prog \<turnstile> (pc, s') \<rightarrow>* (pc', t')" 
+  assumes "prog \<turnstile> (pc, s') \<rightarrow>\<^bsup> k \<^esup> (pc', t')"
+    and "(WHILE ''pc''\<noteq>0 DO GOTO_Prog_to_WHILE_IF prog, s) \<Rightarrow>\<^bsup> (WHILE_complexity prog (pc, s') k) \<^esup> t"
+    and "1 \<le> pc" and "pc \<le> length prog"
     and "well_defined_prog prog"
-    and "(WHILE ''pc''\<noteq>0 DO GOTO_Prog_to_WHILE_IF prog, s) \<Rightarrow>\<^bsup> k \<^esup> t"
     and "s ''pc'' = pc" and "\<forall>x \<noteq> ''pc''. s x = s' x"
   shows "t ''pc'' = pc'" using assms 
-proof (induction "exec1 prog" pc s' pc t rule: star_induct) sorry
+proof (induction prog pc s' k pc' t' arbitrary: s t rule: exec_t_induct)
+  case (step0 P pc s)
+  then show ?case by auto 
+next
+  case (step1 P pc\<^sub>1 s\<^sub>1 pc\<^sub>2 s\<^sub>2 step pc\<^sub>3 s\<^sub>3)
+  have aux1: "1 \<le> pc\<^sub>2 \<and> pc\<^sub>2 \<le> length P" using step1.hyps step1.prems well_defined_prog_pc_range_single by auto
+  have aux2: "iexec (P !! pc\<^sub>1) (pc\<^sub>1, s\<^sub>1) = (pc\<^sub>2, s\<^sub>2)" using step1.hyps(1) exec1_def by auto
+  let ?var = "(case (P !! pc\<^sub>1) of HALT \<Rightarrow> 2 | x ;;= t \<Rightarrow> 4 | x += t \<Rightarrow> 4 | x -= t \<Rightarrow> 4 | 
+      x \<bind>1 \<Rightarrow> 4 | x %=2 \<Rightarrow> 4 | GOTO i \<Rightarrow> 2 | IF x\<noteq>0 THEN GOTO i \<Rightarrow> 3)"
+  have aux3: "(WHILE ''pc''\<noteq>0 DO GOTO_Prog_to_WHILE_IF P, s) \<Rightarrow>\<^bsup> WHILE_complexity P (pc\<^sub>2, s\<^sub>2) step + 5 * pc\<^sub>1 + ?var + 1 \<^esup> t" 
+    using aux2 step1.prems(1) by auto
+  show ?case using step1
+  proof (cases "P !! pc\<^sub>1")
+    case HALT
+    have "\<exists>s'. (GOTO_Prog_to_WHILE_IF P, s) \<Rightarrow>\<^bsup> 5 * pc\<^sub>1 + 2 \<^esup> s'" using step1.hyps(2) HALT aux2 by auto
+    then obtain s' where aux_i: "(GOTO_Prog_to_WHILE_IF P, s) \<Rightarrow>\<^bsup> 5 * pc\<^sub>1 + 2 \<^esup> s'" by blast
+    hence aux4: "(WHILE ''pc''\<noteq>0 DO GOTO_Prog_to_WHILE_IF P, s') \<Rightarrow>\<^bsup> WHILE_complexity P (pc\<^sub>2, s\<^sub>2) step \<^esup> t" 
+      using step1.hyps(2) HALT aux2 by auto 
+    have "s' ''pc'' = pc\<^sub>2 \<and> (\<forall>x. x \<noteq> ''pc'' \<longrightarrow> s' x = s\<^sub>2 x)"
+      using step1.hyps(2) HALT aux2 by auto
+    thus ?thesis using HALT step1 using aux2 by fastforce
+  next
+    case (ASSIGN x c)
+    have aux5: "\<exists>s'. (GOTO_Instr_to_WHILE (x ;;= c), s) \<Rightarrow>\<^bsup> 4 \<^esup> s'" using instr_assign_complexity by auto
+    hence aux6: "\<exists>s'. (GOTO_Prog_to_WHILE_IF P, s) \<Rightarrow>\<^bsup> 5 * pc\<^sub>1 + 4 \<^esup> s'" using GOTO_Prog_to_WHILE_IF_correctness_complexity' by (metis step1.prems(2) step1.prems(3) step1.prems(5) ASSIGN add.commute mult.commute)
+    then obtain s' where aux_i: "(GOTO_Prog_to_WHILE_IF P, s) \<Rightarrow>\<^bsup> 5 * pc\<^sub>1 + 4 \<^esup> s'" by blast
+    hence aux4: "(WHILE ''pc''\<noteq>0 DO GOTO_Prog_to_WHILE_IF P, s') \<Rightarrow>\<^bsup> WHILE_complexity P (pc\<^sub>2, s\<^sub>2) step \<^esup> t" by (smt (verit) step1.prems(2) step1.prems(5) ASSIGN One_nat_def While_tE_time aux3 add.commute add_diff_cancel_right' bigstepT_the_cost bigstepT_the_state diff_diff_left instr.simps(65) le_zero_eq not_less_eq_eq plus_1_eq_Suc)
+    have "s' ''pc'' = pc\<^sub>2 \<and> (\<forall>x. x \<noteq> ''pc'' \<longrightarrow> s' x = s\<^sub>2 x)" by (smt (verit, ccfv_SIG) step1(1) step1(10) step1(7) step1(8) step1(9) step1.prems(2) ASSIGN GOTO_Prog_to_WHILE_IF_correctness_complexity aux5 aux_i bigstepT_the_cost prog_if_pc_consist prog_if_var_consist)
+    thus ?thesis using ASSIGN step1 aux1 aux4 by presburger
+  next
+    case (ADD x c)
+    have aux5: "\<exists>s'. (GOTO_Instr_to_WHILE (x += c), s) \<Rightarrow>\<^bsup> 4 \<^esup> s'" using instr_add_complexity by auto
+    hence aux6: "\<exists>s'. (GOTO_Prog_to_WHILE_IF P, s) \<Rightarrow>\<^bsup> 5 * pc\<^sub>1 + 4 \<^esup> s'" using GOTO_Prog_to_WHILE_IF_correctness_complexity' by (metis step1.prems(2) step1.prems(3) step1.prems(5) ADD add.commute mult.commute)
+    then obtain s' where aux_i: "(GOTO_Prog_to_WHILE_IF P, s) \<Rightarrow>\<^bsup> 5 * pc\<^sub>1 + 4 \<^esup> s'" by blast
+    hence aux4: "(WHILE ''pc''\<noteq>0 DO GOTO_Prog_to_WHILE_IF P, s') \<Rightarrow>\<^bsup> WHILE_complexity P (pc\<^sub>2, s\<^sub>2) step \<^esup> t" by (smt (verit, ccfv_threshold) step1.prems(2) step1.prems(5) ADD One_nat_def While_tE_time add.commute add_diff_cancel_left' aux3 bigstepT_the_cost bigstepT_the_state diff_diff_left instr.simps(66) le_zero_eq not_less_eq_eq plus_1_eq_Suc)
+    have "s' ''pc'' = pc\<^sub>2 \<and> (\<forall>x. x \<noteq> ''pc'' \<longrightarrow> s' x = s\<^sub>2 x)" by (smt (verit, ccfv_SIG) step1(1) step1(10) step1(7) step1(8) step1(9) step1.prems(2) ADD GOTO_Prog_to_WHILE_IF_correctness_complexity aux5 aux_i bigstepT_the_cost prog_if_pc_consist prog_if_var_consist)
+    thus ?thesis using ADD step1 aux1 aux4 by presburger
+  next
+    case (SUB x c)
+    have aux5: "\<exists>s'. (GOTO_Instr_to_WHILE (x -= c), s) \<Rightarrow>\<^bsup> 4 \<^esup> s'" using instr_sub_complexity by auto
+    hence aux6: "\<exists>s'. (GOTO_Prog_to_WHILE_IF P, s) \<Rightarrow>\<^bsup> 5 * pc\<^sub>1 + 4 \<^esup> s'" using GOTO_Prog_to_WHILE_IF_correctness_complexity' by (metis step1.prems(2) step1.prems(3) step1.prems(5) SUB add.commute mult.commute)
+    then obtain s' where aux_i: "(GOTO_Prog_to_WHILE_IF P, s) \<Rightarrow>\<^bsup> 5 * pc\<^sub>1 + 4 \<^esup> s'" by blast
+    hence aux4: "(WHILE ''pc''\<noteq>0 DO GOTO_Prog_to_WHILE_IF P, s') \<Rightarrow>\<^bsup> WHILE_complexity P (pc\<^sub>2, s\<^sub>2) step \<^esup> t" by (smt (verit, ccfv_threshold) step1.prems(2) step1.prems(5) One_nat_def SUB While_tE_time add.commute add_diff_cancel_left' aux3 bigstepT_the_cost bigstepT_the_state diff_diff_left instr.simps(67) le_zero_eq not_less_eq_eq plus_1_eq_Suc)
+    have "s' ''pc'' = pc\<^sub>2 \<and> (\<forall>x. x \<noteq> ''pc'' \<longrightarrow> s' x = s\<^sub>2 x)" by (smt (verit, ccfv_SIG) step1(1) step1(10) step1(7) step1(8) step1(9) step1.prems(2) SUB GOTO_Prog_to_WHILE_IF_correctness_complexity aux5 aux_i bigstepT_the_cost prog_if_pc_consist prog_if_var_consist)
+    thus ?thesis using SUB step1 aux1 aux4 by presburger
+  next
+    case (RSH x)
+    have aux5: "\<exists>s'. (GOTO_Instr_to_WHILE (x \<bind>1), s) \<Rightarrow>\<^bsup> 4 \<^esup> s'" using instr_right_shift_complexity by auto
+    hence aux6: "\<exists>s'. (GOTO_Prog_to_WHILE_IF P, s) \<Rightarrow>\<^bsup> 5 * pc\<^sub>1 + 4 \<^esup> s'" using GOTO_Prog_to_WHILE_IF_correctness_complexity' by (metis step1.prems(2) step1.prems(3) step1.prems(5) RSH add.commute mult.commute)
+    then obtain s' where aux_i: "(GOTO_Prog_to_WHILE_IF P, s) \<Rightarrow>\<^bsup> 5 * pc\<^sub>1 + 4 \<^esup> s'" by blast
+    hence aux4: "(WHILE ''pc''\<noteq>0 DO GOTO_Prog_to_WHILE_IF P, s') \<Rightarrow>\<^bsup> WHILE_complexity P (pc\<^sub>2, s\<^sub>2) step \<^esup> t" by (smt (verit, del_insts) step1.prems(2) step1.prems(5) One_nat_def RSH While_tE_time add.commute add_diff_cancel_right' aux3 bigstepT_the_cost bigstepT_the_state diff_diff_left instr.simps(68) le_zero_eq not_less_eq_eq plus_1_eq_Suc)
+    have "s' ''pc'' = pc\<^sub>2 \<and> (\<forall>x. x \<noteq> ''pc'' \<longrightarrow> s' x = s\<^sub>2 x)" by (smt (verit, ccfv_SIG) step1(1) step1(10) step1(7) step1(8) step1(9) step1.prems(2) RSH GOTO_Prog_to_WHILE_IF_correctness_complexity aux5 aux_i bigstepT_the_cost prog_if_pc_consist prog_if_var_consist)
+    thus ?thesis using RSH step1 aux1 aux4 by presburger
+  next
+    case (MOD x)
+    have aux5: "\<exists>s'. (GOTO_Instr_to_WHILE (x %=2), s) \<Rightarrow>\<^bsup> 4 \<^esup> s'" using instr_right_shift_complexity by auto
+    hence aux6: "\<exists>s'. (GOTO_Prog_to_WHILE_IF P, s) \<Rightarrow>\<^bsup> 5 * pc\<^sub>1 + 4 \<^esup> s'" using GOTO_Prog_to_WHILE_IF_correctness_complexity' by (metis step1.prems(2) step1.prems(3) step1.prems(5) MOD add.commute mult.commute)
+    then obtain s' where aux_i: "(GOTO_Prog_to_WHILE_IF P, s) \<Rightarrow>\<^bsup> 5 * pc\<^sub>1 + 4 \<^esup> s'" by blast
+    hence aux4: "(WHILE ''pc''\<noteq>0 DO GOTO_Prog_to_WHILE_IF P, s') \<Rightarrow>\<^bsup> WHILE_complexity P (pc\<^sub>2, s\<^sub>2) step \<^esup> t" by (smt (verit, ccfv_SIG) step1.prems(2) step1.prems(5) MOD One_nat_def While_tE_time add.commute add_diff_cancel_left' aux3 bigstepT_the_cost bigstepT_the_state diff_diff_left instr.simps(69) le_zero_eq not_less_eq_eq plus_1_eq_Suc)
+    have "s' ''pc'' = pc\<^sub>2 \<and> (\<forall>x. x \<noteq> ''pc'' \<longrightarrow> s' x = s\<^sub>2 x)" by (smt (verit, ccfv_SIG) step1(1) step1(10) step1(7) step1(8) step1(9) step1.prems(2) MOD GOTO_Prog_to_WHILE_IF_correctness_complexity aux5 aux_i bigstepT_the_cost prog_if_pc_consist prog_if_var_consist)
+    thus ?thesis using MOD step1 aux1 aux4 by presburger
+  next
+    case (JMP i)
+    have aux5: "\<exists>s'. (GOTO_Instr_to_WHILE (GOTO i), s) \<Rightarrow>\<^bsup> 2 \<^esup> s'" using instr_jump_complexity by auto
+    hence aux6: "\<exists>s'. (GOTO_Prog_to_WHILE_IF P, s) \<Rightarrow>\<^bsup> 5 * pc\<^sub>1 + 2 \<^esup> s'" using GOTO_Prog_to_WHILE_IF_correctness_complexity' by (metis step1.prems(2) step1.prems(3) step1.prems(5) JMP add.commute mult.commute)
+    then obtain s' where aux_i: "(GOTO_Prog_to_WHILE_IF P, s) \<Rightarrow>\<^bsup> 5 * pc\<^sub>1 + 2 \<^esup> s'" by blast
+    hence aux4: "(WHILE ''pc''\<noteq>0 DO GOTO_Prog_to_WHILE_IF P, s') \<Rightarrow>\<^bsup> WHILE_complexity P (pc\<^sub>2, s\<^sub>2) step \<^esup> t" by (smt (verit, del_insts) step1.prems(2) step1.prems(5) JMP One_nat_def While_tE_time add.commute add_diff_cancel_right' aux3 bigstepT_the_cost bigstepT_the_state diff_diff_left instr.simps(70) le_zero_eq not_less_eq_eq plus_1_eq_Suc)
+    have "s' ''pc'' = pc\<^sub>2 \<and> (\<forall>x. x \<noteq> ''pc'' \<longrightarrow> s' x = s\<^sub>2 x)" by (smt (verit, ccfv_SIG) step1(1) step1(10) step1(7) step1(8) step1(9) step1.prems(2) JMP GOTO_Prog_to_WHILE_IF_correctness_complexity aux5 aux_i bigstepT_the_cost prog_if_pc_consist prog_if_var_consist)
+    thus ?thesis using JMP step1 aux1 aux4 by presburger
+  next
+    case (CONDJMP x i)
+    have aux5: "\<exists>s'. (GOTO_Instr_to_WHILE (IF x\<noteq>0 THEN GOTO i), s) \<Rightarrow>\<^bsup> 3 \<^esup> s'" using instr_cond_jump_complexity by auto
+    hence aux6: "\<exists>s'. (GOTO_Prog_to_WHILE_IF P, s) \<Rightarrow>\<^bsup> 5 * pc\<^sub>1 + 3 \<^esup> s'" using GOTO_Prog_to_WHILE_IF_correctness_complexity' by (metis step1.prems(2) step1.prems(3) step1.prems(5) CONDJMP add.commute mult.commute)
+    then obtain s' where aux_i: "(GOTO_Prog_to_WHILE_IF P, s) \<Rightarrow>\<^bsup> 5 * pc\<^sub>1 + 3 \<^esup> s'" by blast
+    hence aux4: "(WHILE ''pc''\<noteq>0 DO GOTO_Prog_to_WHILE_IF P, s') \<Rightarrow>\<^bsup> WHILE_complexity P (pc\<^sub>2, s\<^sub>2) step \<^esup> t" by (smt (verit) step1.prems(2) step1.prems(5) CONDJMP One_nat_def While_tE_time add.commute add_diff_cancel_left' aux3 bigstepT_the_cost bigstepT_the_state diff_diff_left instr.simps(71) le_zero_eq not_less_eq_eq plus_1_eq_Suc)
+    have "s' ''pc'' = pc\<^sub>2 \<and> (\<forall>x. x \<noteq> ''pc'' \<longrightarrow> s' x = s\<^sub>2 x)" by (smt (verit, ccfv_SIG) step1(1) step1(10) step1(7) step1(8) step1(9) step1.prems(2) CONDJMP GOTO_Prog_to_WHILE_IF_correctness_complexity aux5 aux_i bigstepT_the_cost prog_if_pc_consist prog_if_var_consist)
+    thus ?thesis using CONDJMP step1 aux1 aux4 by presburger
+  qed
+qed
+
+lemma prog_var_consist:
+  assumes "prog \<turnstile> (pc, s') \<rightarrow>\<^bsup> k \<^esup> (pc', t')"
+    and "(WHILE ''pc''\<noteq>0 DO GOTO_Prog_to_WHILE_IF prog, s) \<Rightarrow>\<^bsup> (WHILE_complexity prog (pc, s') k) \<^esup> t"
+    and "1 \<le> pc" and "pc \<le> length prog"
+    and "well_defined_prog prog"
+    and "s ''pc'' = pc" and "\<forall>x \<noteq> ''pc''. s x = s' x"
+  shows "\<forall>x \<noteq> ''pc''. t x = t' x" using assms 
+proof (induction prog pc s' k pc' t' arbitrary: s t rule: exec_t_induct)
+  case (step0 P pc s)
+  then show ?case by auto 
+next
+  case (step1 P pc\<^sub>1 s\<^sub>1 pc\<^sub>2 s\<^sub>2 step pc\<^sub>3 s\<^sub>3)
+  have aux1: "1 \<le> pc\<^sub>2 \<and> pc\<^sub>2 \<le> length P" using step1.hyps step1.prems well_defined_prog_pc_range_single by auto
+  have aux2: "iexec (P !! pc\<^sub>1) (pc\<^sub>1, s\<^sub>1) = (pc\<^sub>2, s\<^sub>2)" using step1.hyps(1) exec1_def by auto
+  let ?var = "(case (P !! pc\<^sub>1) of HALT \<Rightarrow> 2 | x ;;= t \<Rightarrow> 4 | x += t \<Rightarrow> 4 | x -= t \<Rightarrow> 4 | 
+      x \<bind>1 \<Rightarrow> 4 | x %=2 \<Rightarrow> 4 | GOTO i \<Rightarrow> 2 | IF x\<noteq>0 THEN GOTO i \<Rightarrow> 3)"
+  have aux3: "(WHILE ''pc''\<noteq>0 DO GOTO_Prog_to_WHILE_IF P, s) \<Rightarrow>\<^bsup> WHILE_complexity P (pc\<^sub>2, s\<^sub>2) step + 5 * pc\<^sub>1 + ?var + 1 \<^esup> t" 
+    using aux2 step1.prems(1) by auto
+  show ?case using step1
+  proof (cases "P !! pc\<^sub>1")
+    case HALT
+    have "\<exists>s'. (GOTO_Prog_to_WHILE_IF P, s) \<Rightarrow>\<^bsup> 5 * pc\<^sub>1 + 2 \<^esup> s'" using step1.hyps(2) HALT aux2 by auto
+    then obtain s' where aux_i: "(GOTO_Prog_to_WHILE_IF P, s) \<Rightarrow>\<^bsup> 5 * pc\<^sub>1 + 2 \<^esup> s'" by blast
+    hence aux4: "(WHILE ''pc''\<noteq>0 DO GOTO_Prog_to_WHILE_IF P, s') \<Rightarrow>\<^bsup> WHILE_complexity P (pc\<^sub>2, s\<^sub>2) step \<^esup> t" 
+      using step1.hyps(2) HALT aux2 by auto 
+    have "s' ''pc'' = pc\<^sub>2 \<and> (\<forall>x. x \<noteq> ''pc'' \<longrightarrow> s' x = s\<^sub>2 x)"
+      using step1.hyps(2) HALT aux2 by auto
+    thus ?thesis using HALT step1 using aux2 by fastforce
+  next
+    case (ASSIGN x c)
+    have aux5: "\<exists>s'. (GOTO_Instr_to_WHILE (x ;;= c), s) \<Rightarrow>\<^bsup> 4 \<^esup> s'" using instr_assign_complexity by auto
+    hence aux6: "\<exists>s'. (GOTO_Prog_to_WHILE_IF P, s) \<Rightarrow>\<^bsup> 5 * pc\<^sub>1 + 4 \<^esup> s'" using GOTO_Prog_to_WHILE_IF_correctness_complexity' by (metis step1.prems(2) step1.prems(3) step1.prems(5) ASSIGN add.commute mult.commute)
+    then obtain s' where aux_i: "(GOTO_Prog_to_WHILE_IF P, s) \<Rightarrow>\<^bsup> 5 * pc\<^sub>1 + 4 \<^esup> s'" by blast
+    hence aux4: "(WHILE ''pc''\<noteq>0 DO GOTO_Prog_to_WHILE_IF P, s') \<Rightarrow>\<^bsup> WHILE_complexity P (pc\<^sub>2, s\<^sub>2) step \<^esup> t" by (smt (verit) step1.prems(2) step1.prems(5) ASSIGN One_nat_def While_tE_time aux3 add.commute add_diff_cancel_right' bigstepT_the_cost bigstepT_the_state diff_diff_left instr.simps(65) le_zero_eq not_less_eq_eq plus_1_eq_Suc)
+    have "s' ''pc'' = pc\<^sub>2 \<and> (\<forall>x. x \<noteq> ''pc'' \<longrightarrow> s' x = s\<^sub>2 x)" by (smt (verit, ccfv_SIG) step1(1) step1(10) step1(7) step1(8) step1(9) step1.prems(2) ASSIGN GOTO_Prog_to_WHILE_IF_correctness_complexity aux5 aux_i bigstepT_the_cost prog_if_pc_consist prog_if_var_consist)
+    thus ?thesis using ASSIGN step1 aux1 aux4 by presburger
+  next
+    case (ADD x c)
+    have aux5: "\<exists>s'. (GOTO_Instr_to_WHILE (x += c), s) \<Rightarrow>\<^bsup> 4 \<^esup> s'" using instr_add_complexity by auto
+    hence aux6: "\<exists>s'. (GOTO_Prog_to_WHILE_IF P, s) \<Rightarrow>\<^bsup> 5 * pc\<^sub>1 + 4 \<^esup> s'" using GOTO_Prog_to_WHILE_IF_correctness_complexity' by (metis step1.prems(2) step1.prems(3) step1.prems(5) ADD add.commute mult.commute)
+    then obtain s' where aux_i: "(GOTO_Prog_to_WHILE_IF P, s) \<Rightarrow>\<^bsup> 5 * pc\<^sub>1 + 4 \<^esup> s'" by blast
+    hence aux4: "(WHILE ''pc''\<noteq>0 DO GOTO_Prog_to_WHILE_IF P, s') \<Rightarrow>\<^bsup> WHILE_complexity P (pc\<^sub>2, s\<^sub>2) step \<^esup> t" by (smt (verit, ccfv_threshold) step1.prems(2) step1.prems(5) ADD One_nat_def While_tE_time add.commute add_diff_cancel_left' aux3 bigstepT_the_cost bigstepT_the_state diff_diff_left instr.simps(66) le_zero_eq not_less_eq_eq plus_1_eq_Suc)
+    have "s' ''pc'' = pc\<^sub>2 \<and> (\<forall>x. x \<noteq> ''pc'' \<longrightarrow> s' x = s\<^sub>2 x)" by (smt (verit, ccfv_SIG) step1(1) step1(10) step1(7) step1(8) step1(9) step1.prems(2) ADD GOTO_Prog_to_WHILE_IF_correctness_complexity aux5 aux_i bigstepT_the_cost prog_if_pc_consist prog_if_var_consist)
+    thus ?thesis using ADD step1 aux1 aux4 by presburger
+  next
+    case (SUB x c)
+    have aux5: "\<exists>s'. (GOTO_Instr_to_WHILE (x -= c), s) \<Rightarrow>\<^bsup> 4 \<^esup> s'" using instr_sub_complexity by auto
+    hence aux6: "\<exists>s'. (GOTO_Prog_to_WHILE_IF P, s) \<Rightarrow>\<^bsup> 5 * pc\<^sub>1 + 4 \<^esup> s'" using GOTO_Prog_to_WHILE_IF_correctness_complexity' by (metis step1.prems(2) step1.prems(3) step1.prems(5) SUB add.commute mult.commute)
+    then obtain s' where aux_i: "(GOTO_Prog_to_WHILE_IF P, s) \<Rightarrow>\<^bsup> 5 * pc\<^sub>1 + 4 \<^esup> s'" by blast
+    hence aux4: "(WHILE ''pc''\<noteq>0 DO GOTO_Prog_to_WHILE_IF P, s') \<Rightarrow>\<^bsup> WHILE_complexity P (pc\<^sub>2, s\<^sub>2) step \<^esup> t" by (smt (verit, ccfv_threshold) step1.prems(2) step1.prems(5) One_nat_def SUB While_tE_time add.commute add_diff_cancel_left' aux3 bigstepT_the_cost bigstepT_the_state diff_diff_left instr.simps(67) le_zero_eq not_less_eq_eq plus_1_eq_Suc)
+    have "s' ''pc'' = pc\<^sub>2 \<and> (\<forall>x. x \<noteq> ''pc'' \<longrightarrow> s' x = s\<^sub>2 x)" by (smt (verit, ccfv_SIG) step1(1) step1(10) step1(7) step1(8) step1(9) step1.prems(2) SUB GOTO_Prog_to_WHILE_IF_correctness_complexity aux5 aux_i bigstepT_the_cost prog_if_pc_consist prog_if_var_consist)
+    thus ?thesis using SUB step1 aux1 aux4 by presburger
+  next
+    case (RSH x)
+    have aux5: "\<exists>s'. (GOTO_Instr_to_WHILE (x \<bind>1), s) \<Rightarrow>\<^bsup> 4 \<^esup> s'" using instr_right_shift_complexity by auto
+    hence aux6: "\<exists>s'. (GOTO_Prog_to_WHILE_IF P, s) \<Rightarrow>\<^bsup> 5 * pc\<^sub>1 + 4 \<^esup> s'" using GOTO_Prog_to_WHILE_IF_correctness_complexity' by (metis step1.prems(2) step1.prems(3) step1.prems(5) RSH add.commute mult.commute)
+    then obtain s' where aux_i: "(GOTO_Prog_to_WHILE_IF P, s) \<Rightarrow>\<^bsup> 5 * pc\<^sub>1 + 4 \<^esup> s'" by blast
+    hence aux4: "(WHILE ''pc''\<noteq>0 DO GOTO_Prog_to_WHILE_IF P, s') \<Rightarrow>\<^bsup> WHILE_complexity P (pc\<^sub>2, s\<^sub>2) step \<^esup> t" by (smt (verit, del_insts) step1.prems(2) step1.prems(5) One_nat_def RSH While_tE_time add.commute add_diff_cancel_right' aux3 bigstepT_the_cost bigstepT_the_state diff_diff_left instr.simps(68) le_zero_eq not_less_eq_eq plus_1_eq_Suc)
+    have "s' ''pc'' = pc\<^sub>2 \<and> (\<forall>x. x \<noteq> ''pc'' \<longrightarrow> s' x = s\<^sub>2 x)" by (smt (verit, ccfv_SIG) step1(1) step1(10) step1(7) step1(8) step1(9) step1.prems(2) RSH GOTO_Prog_to_WHILE_IF_correctness_complexity aux5 aux_i bigstepT_the_cost prog_if_pc_consist prog_if_var_consist)
+    thus ?thesis using RSH step1 aux1 aux4 by presburger
+  next
+    case (MOD x)
+    have aux5: "\<exists>s'. (GOTO_Instr_to_WHILE (x %=2), s) \<Rightarrow>\<^bsup> 4 \<^esup> s'" using instr_right_shift_complexity by auto
+    hence aux6: "\<exists>s'. (GOTO_Prog_to_WHILE_IF P, s) \<Rightarrow>\<^bsup> 5 * pc\<^sub>1 + 4 \<^esup> s'" using GOTO_Prog_to_WHILE_IF_correctness_complexity' by (metis step1.prems(2) step1.prems(3) step1.prems(5) MOD add.commute mult.commute)
+    then obtain s' where aux_i: "(GOTO_Prog_to_WHILE_IF P, s) \<Rightarrow>\<^bsup> 5 * pc\<^sub>1 + 4 \<^esup> s'" by blast
+    hence aux4: "(WHILE ''pc''\<noteq>0 DO GOTO_Prog_to_WHILE_IF P, s') \<Rightarrow>\<^bsup> WHILE_complexity P (pc\<^sub>2, s\<^sub>2) step \<^esup> t" by (smt (verit, ccfv_SIG) step1.prems(2) step1.prems(5) MOD One_nat_def While_tE_time add.commute add_diff_cancel_left' aux3 bigstepT_the_cost bigstepT_the_state diff_diff_left instr.simps(69) le_zero_eq not_less_eq_eq plus_1_eq_Suc)
+    have "s' ''pc'' = pc\<^sub>2 \<and> (\<forall>x. x \<noteq> ''pc'' \<longrightarrow> s' x = s\<^sub>2 x)" by (smt (verit, ccfv_SIG) step1(1) step1(10) step1(7) step1(8) step1(9) step1.prems(2) MOD GOTO_Prog_to_WHILE_IF_correctness_complexity aux5 aux_i bigstepT_the_cost prog_if_pc_consist prog_if_var_consist)
+    thus ?thesis using MOD step1 aux1 aux4 by presburger
+  next
+    case (JMP i)
+    have aux5: "\<exists>s'. (GOTO_Instr_to_WHILE (GOTO i), s) \<Rightarrow>\<^bsup> 2 \<^esup> s'" using instr_jump_complexity by auto
+    hence aux6: "\<exists>s'. (GOTO_Prog_to_WHILE_IF P, s) \<Rightarrow>\<^bsup> 5 * pc\<^sub>1 + 2 \<^esup> s'" using GOTO_Prog_to_WHILE_IF_correctness_complexity' by (metis step1.prems(2) step1.prems(3) step1.prems(5) JMP add.commute mult.commute)
+    then obtain s' where aux_i: "(GOTO_Prog_to_WHILE_IF P, s) \<Rightarrow>\<^bsup> 5 * pc\<^sub>1 + 2 \<^esup> s'" by blast
+    hence aux4: "(WHILE ''pc''\<noteq>0 DO GOTO_Prog_to_WHILE_IF P, s') \<Rightarrow>\<^bsup> WHILE_complexity P (pc\<^sub>2, s\<^sub>2) step \<^esup> t" by (smt (verit, del_insts) step1.prems(2) step1.prems(5) JMP One_nat_def While_tE_time add.commute add_diff_cancel_right' aux3 bigstepT_the_cost bigstepT_the_state diff_diff_left instr.simps(70) le_zero_eq not_less_eq_eq plus_1_eq_Suc)
+    have "s' ''pc'' = pc\<^sub>2 \<and> (\<forall>x. x \<noteq> ''pc'' \<longrightarrow> s' x = s\<^sub>2 x)" by (smt (verit, ccfv_SIG) step1(1) step1(10) step1(7) step1(8) step1(9) step1.prems(2) JMP GOTO_Prog_to_WHILE_IF_correctness_complexity aux5 aux_i bigstepT_the_cost prog_if_pc_consist prog_if_var_consist)
+    thus ?thesis using JMP step1 aux1 aux4 by presburger
+  next
+    case (CONDJMP x i)
+    have aux5: "\<exists>s'. (GOTO_Instr_to_WHILE (IF x\<noteq>0 THEN GOTO i), s) \<Rightarrow>\<^bsup> 3 \<^esup> s'" using instr_cond_jump_complexity by auto
+    hence aux6: "\<exists>s'. (GOTO_Prog_to_WHILE_IF P, s) \<Rightarrow>\<^bsup> 5 * pc\<^sub>1 + 3 \<^esup> s'" using GOTO_Prog_to_WHILE_IF_correctness_complexity' by (metis step1.prems(2) step1.prems(3) step1.prems(5) CONDJMP add.commute mult.commute)
+    then obtain s' where aux_i: "(GOTO_Prog_to_WHILE_IF P, s) \<Rightarrow>\<^bsup> 5 * pc\<^sub>1 + 3 \<^esup> s'" by blast
+    hence aux4: "(WHILE ''pc''\<noteq>0 DO GOTO_Prog_to_WHILE_IF P, s') \<Rightarrow>\<^bsup> WHILE_complexity P (pc\<^sub>2, s\<^sub>2) step \<^esup> t" by (smt (verit) step1.prems(2) step1.prems(5) CONDJMP One_nat_def While_tE_time add.commute add_diff_cancel_left' aux3 bigstepT_the_cost bigstepT_the_state diff_diff_left instr.simps(71) le_zero_eq not_less_eq_eq plus_1_eq_Suc)
+    have "s' ''pc'' = pc\<^sub>2 \<and> (\<forall>x. x \<noteq> ''pc'' \<longrightarrow> s' x = s\<^sub>2 x)" by (smt (verit, ccfv_SIG) step1(1) step1(10) step1(7) step1(8) step1(9) step1.prems(2) CONDJMP GOTO_Prog_to_WHILE_IF_correctness_complexity aux5 aux_i bigstepT_the_cost prog_if_pc_consist prog_if_var_consist)
+    thus ?thesis using CONDJMP step1 aux1 aux4 by presburger
+  qed
+qed
+
+lemma prog_complexity:
+  assumes "prog \<turnstile> (pc, s') \<rightarrow>\<^bsup> k \<^esup> (pc', t')"
+    and "1 \<le> pc" and "pc \<le> length prog"
+    and "well_defined_prog prog"
+    and "s ''pc'' = pc" and "\<forall>x \<noteq> ''pc''. s x = s' x"
+  shows "\<exists>t. (WHILE ''pc''\<noteq>0 DO GOTO_Prog_to_WHILE_IF prog, s) \<Rightarrow>\<^bsup> (WHILE_complexity prog (pc, s') k) \<^esup> t" using assms
+proof (induction prog pc s' k pc' t' arbitrary: s rule: exec_t_induct)
+  case (step0 P pc s1)
+  (*not provable because no bit step matches with complexity 0*)
+  then show ?case sorry
+next
+  case (step1 P pc\<^sub>1 s\<^sub>1 pc\<^sub>2 s\<^sub>2 k pc\<^sub>3 s\<^sub>3)
+  then show ?case sorry
+qed
+
+lemma prog_complexity':
+  assumes "prog \<turnstile> (pc, s') \<rightarrow>\<^bsup> k \<^esup> (pc', t')"
+    and "1 \<le> pc" and "pc \<le> length prog" and "k > 0"
+    and "well_defined_prog prog"
+    and "s ''pc'' = pc" and "\<forall>x \<noteq> ''pc''. s x = s' x"
+  shows "\<exists>t. (WHILE ''pc''\<noteq>0 DO GOTO_Prog_to_WHILE_IF prog, s) \<Rightarrow>\<^bsup> (WHILE_complexity prog (pc, s') k) \<^esup> t" using assms
+proof (induction prog pc s' k pc' t' arbitrary: s rule: exec_t_induct)
+  case (step0 P pc s1)
+  then show ?case by blast
+next
+  case (step1 P pc\<^sub>1 s\<^sub>1 pc\<^sub>2 s\<^sub>2 k pc\<^sub>3 s\<^sub>3)
+  (* not provable because this step relies on the big step with complexity 0 *)
+  then show ?case sorry
+qed
+
+(*
+  GOTO Program can have 0 step, but big step cannot \<Longrightarrow> prog_complexity problem above
+*)
+
+(*
+  Since SKIP is the only big step which has complexity 1
+  \<Longrightarrow>
+  If a big step has complexity 1, then it must be SKIP
+*)
+lemma "(c, s) \<Rightarrow>\<^bsup> 1 \<^esup> t \<Longrightarrow> c = SKIP"
+  apply (cases c)
+  apply simp
+  apply (metis Assign_tE One_nat_def n_not_Suc_n)
+  apply (metis One_nat_def Seq_tE add_is_1 bigstep_progress less_numeral_extra(3))
+  using bigstep_progress apply fastforce
+  by auto
+
+(*
+  A solution to solve prog_complexity problem is to add another big step rule which is:
+  NotRun: (Empty, s) \<Rightarrow>\<^bsup> 0 \<^esup> t
+
+  And then using the above lemma to reversely get the big step runs 0 step.
+*)
+
+lemma 
+assumes "prog \<turnstile> (pc, s') \<rightarrow>\<^bsup> k \<^esup> (pc', t')"
+    and "(GOTO_Prog_to_WHILE prog, s) \<Rightarrow>\<^bsup> 2 + (WHILE_complexity prog (pc, s') k) \<^esup> t"
+    and "well_defined_prog prog" and "pc = 1"
+    and "\<forall>x \<noteq> ''pc''. s x = s' x"
+  shows "\<forall>x \<noteq> ''pc''. t x = t' x" using assms
+proof -
+  have "(''pc'' ::= A (atomExp.N 1), s) \<Rightarrow>\<^bsup> 2 \<^esup> s(''pc'' := 1)" by (simp add: assign_t_simp numeral_2_eq_2)
+  let ?s = "s(''pc'' := 1)"
+  have aux1: "(WHILE ''pc''\<noteq>0 DO GOTO_Prog_to_WHILE_IF prog, ?s) \<Rightarrow>\<^bsup> (WHILE_complexity prog (pc, s') k) \<^esup> t" 
+    using GOTO_Prog_to_WHILE_def assms(2) by fastforce
+  have aux2: "1 \<le> pc" by (simp add: assms(4))
+  have aux3: "pc \<le> length prog" using assms(3) assms(4) well_defined_prog_def by blast
+  have aux4: "?s ''pc'' = pc" by (simp add: assms(4))
+  have aux5: "\<forall>x \<noteq> ''pc''. ?s x = s' x" by (simp add: assms(5))
+  show "\<forall>x \<noteq> ''pc''. t x = t' x" 
+    using prog_var_consist[of prog pc s' k pc' t' ?s t, OF assms(1) aux1 aux2 aux3 assms(3) aux4 aux5] by blast
+qed
+
+lemma 
+assumes "prog \<turnstile> (pc, s') \<rightarrow>\<^bsup> k \<^esup> (pc', t')"
+    and "(GOTO_Prog_to_WHILE prog, s) \<Rightarrow>\<^bsup> 2 + (WHILE_complexity prog (pc, s') k) \<^esup> t"
+    and "well_defined_prog prog" and "pc = 1"
+    and "\<forall>x \<noteq> ''pc''. s x = s' x"
+  shows "t ''pc'' = pc'" using assms
+proof -
+  have "(''pc'' ::= A (atomExp.N 1), s) \<Rightarrow>\<^bsup> 2 \<^esup> s(''pc'' := 1)" by (simp add: assign_t_simp numeral_2_eq_2)
+  let ?s = "s(''pc'' := 1)"
+  have aux1: "(WHILE ''pc''\<noteq>0 DO GOTO_Prog_to_WHILE_IF prog, ?s) \<Rightarrow>\<^bsup> (WHILE_complexity prog (pc, s') k) \<^esup> t" 
+    using GOTO_Prog_to_WHILE_def assms(2) by fastforce
+  have aux2: "1 \<le> pc" by (simp add: assms(4))
+  have aux3: "pc \<le> length prog" using assms(3) assms(4) well_defined_prog_def by blast
+  have aux4: "?s ''pc'' = pc" by (simp add: assms(4))
+  have aux5: "\<forall>x \<noteq> ''pc''. ?s x = s' x" by (simp add: assms(5))
+  show "t ''pc'' = pc'" 
+    using prog_pc_consist[of prog pc s' k pc' t' ?s t, OF assms(1) aux1 aux2 aux3 assms(3) aux4 aux5] by blast
+qed
+
+(*
+
+complexity problem is the same as prog_complexity, need big_step to be fixed.
+
+*)
+
 end
